

# Geometry I: Comprehensive Solutions & Audit

Collins Mwangi  
University of Nairobi

Monday, 15th December 2025

Version 1.0

# 1 Part I: Final Answers Summary

*Use this section to quickly check your results before diving into the workings.*

1. **Equation of Circle:**  $x^2 + y^2 = 25$
2. **Equation of Line:**  $y = -x + 4$  (or  $x + y - 4 = 0$ )
3. **Intersection Points:**  $(2.48, -1.96)$  and  $(-0.08, 3.16)$
4. **Point Position:** The point  $(3, 4)$  lies **OUTSIDE** the circle.
5. **Parallelogram Test:**  $ABCD$  is **NOT** a parallelogram (Opposite sides are unequal).
6. **Intersection Angle:** Acute angle  $\theta \approx 84.61^\circ$  (Obtuse  $\approx 95.39^\circ$ ).
7. **Midpoint:**  $(2, 6)$
8. **Distance Between Lines:** 3 units.
9. **Centre and Radius:** Centre  $(4, 0)$ , Radius  $r \approx 3.61$  units ( $\sqrt{13}$ ).

## 2 Part II: Detailed Worked Solutions

### Question 1: Diameter of a Circle

**Given:** Diameter endpoints  $A(3, -4)$  and  $B(-3, 4)$ .

#### Step-by-Step Derivation

##### Step 1: Find the Centre (Midpoint Formula)

$$M = \left( \frac{x_1 + x_2}{2}, \frac{y_1 + y_2}{2} \right)$$

Substitute  $x_1 = 3, x_2 = -3, y_1 = -4, y_2 = 4$ :

$$M = \left( \frac{3 + (-3)}{2}, \frac{-4 + 4}{2} \right) = \left( \frac{0}{2}, \frac{0}{2} \right) = (0, 0)$$

**Centre:**  $C(0, 0)$ .

##### Step 2: Find the Radius (Distance from Centre to Point A)

$$r = \sqrt{(x_2 - x_1)^2 + (y_2 - y_1)^2}$$

Substitute Centre  $(0, 0)$  and Point  $A(3, -4)$ :

$$r = \sqrt{(3 - 0)^2 + (-4 - 0)^2}$$

$$r = \sqrt{3^2 + (-4)^2} = \sqrt{9 + 16} = \sqrt{25} = 5$$

##### Step 3: Write the Standard Equation

$$(x - h)^2 + (y - k)^2 = r^2$$

Substitute  $h = 0, k = 0, r = 5$ :

$$(x - 0)^2 + (y - 0)^2 = 5^2$$

$$\boxed{x^2 + y^2 = 25}$$

#### Alternative Method: Diameter Form

The equation of a circle with diameter endpoints  $(x_1, y_1)$  and  $(x_2, y_2)$  is:

$$(x - x_1)(x - x_2) + (y - y_1)(y - y_2) = 0$$

Substitute points:

$$(x - 3)(x - (-3)) + (y - (-4))(y - 4) = 0$$

$$(x - 3)(x + 3) + (y + 4)(y - 4) = 0$$

Expand (difference of squares):

$$(x^2 - 9) + (y^2 - 16) = 0$$

$$x^2 + y^2 - 25 = 0 \implies x^2 + y^2 = 25$$

**Question 2: Equation of a Line****Given:** Points  $P_1(-3, 7)$  and  $P_2(5, -1)$ .**Step-by-Step Derivation****Step 1: Calculate Gradient ( $m$ )**

$$m = \frac{y_2 - y_1}{x_2 - x_1} = \frac{-1 - 7}{5 - (-3)}$$

$$m = \frac{-8}{5 + 3} = \frac{-8}{8} = -1$$

**Step 2: Use Point-Slope Form** Using  $P_1(-3, 7)$  and  $m = -1$ :

$$y - y_1 = m(x - x_1)$$

$$y - 7 = -1(x - (-3))$$

$$y - 7 = -1(x + 3)$$

Expand the brackets:

$$y - 7 = -x - 3$$

Add 7 to both sides:

$$y = -x - 3 + 7$$

$$\boxed{y = -x + 4}$$

**Question 3: Line-Circle Intersection****Given:** Line  $2x + y = 3$  and Circle  $x^2 + y^2 = 10$ .**Step-by-Step Derivation****Step 1: Isolate a variable in the linear equation** From  $2x + y = 3$ , subtract  $2x$  from both sides:

$$y = 3 - 2x$$

**Step 2: Substitute into the Circle Equation**

$$x^2 + (3 - 2x)^2 = 10$$

**Step 3: Expand the squared term** Recall  $(a - b)^2 = a^2 - 2ab + b^2$ . Here  $a = 3, b = 2x$ .

$$\begin{aligned}(3 - 2x)^2 &= 3^2 - 2(3)(2x) + (2x)^2 \\ &= 9 - 12x + 4x^2\end{aligned}$$

Substitute back:

$$x^2 + (9 - 12x + 4x^2) = 10$$

**Step 4: Form the Quadratic Equation** Combine like terms ( $x^2 + 4x^2 = 5x^2$ ):

$$5x^2 - 12x + 9 = 10$$

Subtract 10 from both sides:

$$5x^2 - 12x - 1 = 0$$

**Step 5: Solve for  $x$  (Quadratic Formula)**

$$x = \frac{-b \pm \sqrt{b^2 - 4ac}}{2a}$$

$$a = 5, b = -12, c = -1.$$

$$x = \frac{-(-12) \pm \sqrt{(-12)^2 - 4(5)(-1)}}{2(5)}$$

$$x = \frac{12 \pm \sqrt{144 + 20}}{10} = \frac{12 \pm \sqrt{164}}{10}$$

$$\sqrt{164} \approx 12.806$$

$$x_1 = \frac{12 + 12.806}{10} = 2.4806 \quad \text{and} \quad x_2 = \frac{12 - 12.806}{10} = -0.0806$$

**Step 6: Solve for  $y$  Using  $y = 3 - 2x$ :**

- If  $x \approx 2.48$ :  $y = 3 - 2(2.48) = 3 - 4.96 = -1.96$ .
- If  $x \approx -0.08$ :  $y = 3 - 2(-0.08) = 3 + 0.16 = 3.16$ .

**Answers:**  $(2.48, -1.96)$  and  $(-0.08, 3.16)$ .

**Common Error: The Square Root Trap**

**Avoid** writing  $y = \sqrt{10 - x^2}$ . Why? The symbol  $\sqrt{\dots}$  (principal root) only outputs positive numbers. If you use it, you delete the bottom half of the circle ( $y < 0$ ) and will miss the intersection point at  $y = -1.96$ .

## Question 4: Point Position Check

**Goal:** Check if  $(3, 4)$  is inside  $x^2 + y^2 - 14x + 16y = 0$ .

### Step-by-Step Derivation

**Step 1: Evaluate the function at the point** Let  $f(x, y) = x^2 + y^2 - 14x + 16y$ . Substitute  $x = 3, y = 4$ :

$$f(3, 4) = (3)^2 + (4)^2 - 14(3) + 16(4)$$

Calculate terms:

$$\begin{aligned} &= 9 + 16 - 42 + 64 \\ &= 25 - 42 + 64 \\ &= -17 + 64 \\ &= 47 \end{aligned}$$

**Step 2: Interpret the result**

- If result  $< 0$ : Point is Inside.
- If result  $= 0$ : Point is On the Circle.
- If result  $> 0$ : Point is Outside.

Since  $47 > 0$ , the point  $(3, 4)$  is **OUTSIDE** the circle (not inside as may have been expected).

### Question 5: Parallelogram Verification

**Given:**  $A(0, -3)$ ,  $B(5, 0)$ ,  $C(4, -3)$ ,  $D(-4, -1)$ .

#### Step-by-Step Derivation

**Theory:** A parallelogram must have two pairs of equal opposite sides ( $AB = CD$  and  $BC = AD$ ). We only need to disprove one pair to fail the test.

##### Step 1: Length of AB

$$d = \sqrt{(5 - 0)^2 + (0 - (-3))^2} = \sqrt{5^2 + 3^2} = \sqrt{25 + 9} = \sqrt{34} \approx 5.83$$

##### Step 2: Length of CD (Opposite to AB)

$$d = \sqrt{(-4 - 4)^2 + (-1 - (-3))^2} = \sqrt{(-8)^2 + (2)^2} = \sqrt{64 + 4} = \sqrt{68} \approx 8.25$$

**Conclusion:** Since  $\sqrt{34} \neq \sqrt{68}$ , the opposite sides are not equal. Therefore, **ABCD** is not a parallelogram.

### Question 6: Angle of Intersection

**Line 1:**  $(4, 3)$  and  $(-6, 0)$ . **Line 2:**  $(0, 0)$  and  $(-1, 5)$ .

#### Step-by-Step Derivation

##### Step 1: Calculate Gradients

$$m_1 = \frac{0 - 3}{-6 - 4} = \frac{-3}{-10} = 0.3$$

$$m_2 = \frac{5 - 0}{-1 - 0} = \frac{5}{-1} = -5$$

##### Step 2: Apply the Angle Formula

$$\tan \theta = \left| \frac{m_2 - m_1}{1 + m_1 m_2} \right|$$

Substitute values:

$$\text{Numerator} = -5 - 0.3 = -5.3$$

$$\text{Denominator} = 1 + (0.3)(-5) = 1 - 1.5 = -0.5$$

$$\tan \theta = \left| \frac{-5.3}{-0.5} \right| = |10.6| = 10.6$$

##### Step 3: Solve for $\theta$

$$\theta = \tan^{-1}(10.6) \approx 84.61^\circ$$

**Note: Two Angles**

Intersecting lines create two angles that sum to  $180^\circ$ .

- Acute Angle:  $84.61^\circ$  (Found by using absolute value).
- Obtuse Angle:  $180^\circ - 84.61^\circ = 95.39^\circ$ .

**Question 7: Midpoint Calculation**

**Given:**  $A(-7, 12)$  and  $B(11, 0)$ .

**Step-by-Step Derivation**

$$M = \left( \frac{x_1 + x_2}{2}, \frac{y_1 + y_2}{2} \right)$$

Substitute:

$$M = \left( \frac{-7 + 11}{2}, \frac{12 + 0}{2} \right)$$

$$M = \left( \frac{4}{2}, \frac{12}{2} \right)$$

$$M = (2, 6)$$

**Question 8: Distance Between Parallel Lines**

**Lines:**  $L_1 : 4x - 3y - 9 = 0$  and  $L_2 : 4x - 3y - 24 = 0$ .

**Step-by-Step Derivation**

**Step 1: Identify Constants** The lines are in the form  $Ax + By + C = 0$ .  $A = 4$ ,  $B = -3$ .  $C_1 = -9$ ,  $C_2 = -24$ .

**Step 2: Use the Distance Formula**

$$d = \frac{|C_1 - C_2|}{\sqrt{A^2 + B^2}}$$

Substitute:

$$d = \frac{|-9 - (-24)|}{\sqrt{4^2 + (-3)^2}}$$

Simplify numerator (watch the signs!):

$$|-9 + 24| = |15| = 15$$

Simplify denominator:

$$\sqrt{16 + 9} = \sqrt{25} = 5$$

Final Division:

$$d = \frac{15}{5} = 3 \text{ units}$$

**Question 9: Centre and Radius**

**Equation:**  $(x - 4)^2 + y^2 = 13$ .

**Step-by-Step Derivation**

**Step 1: Match with Standard Form** Standard form:  $(x - h)^2 + (y - k)^2 = r^2$ . Given:  $(x - 4)^2 + (y - 0)^2 = 13$ .

**Step 2: Extract Values**  $h = 4, k = 0 \implies$  Centre  $(4, 0)$ .  $r^2 = 13 \implies r = \sqrt{13}$ .

**Step 3: Calculate Radius Value**

$$r = \sqrt{13}$$

$$r \approx 3.60555\dots$$

Round to 2 decimal places:  $\approx 3.61$ .